src/translation/HTLgenproof.v
@@ -390,7 +390,7 @@ Section CORRECTNESS.
   Lemma op_stack_based :
     forall F V sp v m args rs op ge pc' res0 pc f e fin rtrn st stk,
       tr_instr fin rtrn st stk (RTL.Iop op args res0 pc')
-               (Verilog.Vnonblock (Verilog.Vvar res0) e)
+               (vstmnt (Verilog.Vnonblock (Verilog.Vvar res0) e))
                (state_goto st pc') ->
       reg_stack_based_pointers sp rs ->
       (RTL.fn_code f) ! pc = Some (RTL.Iop op args res0 pc') ->
@@ -971,6 +971,7 @@ Section CORRECTNESS.
     econstructor.
     econstructor.
     econstructor.
+    econstructor.
 
     all: invert MARR; big_tac.
 
@@ -992,6 +993,7 @@ Section CORRECTNESS.
           Smallstep.plus HTL.step tge R1 Events.E0 R2 /\
           match_states (RTL.State s f sp pc' (Registers.Regmap.set res0 v rs) m) R2.
   Proof.
+    (*
     intros s f sp pc rs m op args res0 pc' v H H0 R1 MSTATE.
     inv_state. inv MARR.
     exploit eval_correct; eauto. intros. inversion H1. inversion H2.
@@ -1029,7 +1031,8 @@ Section CORRECTNESS.
       by (eapply RTL.max_reg_function_def; eauto; simpl; auto).
     unfold Ple in HPle. lia.
     Unshelve. exact tt.
-  Qed.
+    *)
+  Admitted.
   Hint Resolve transl_iop_correct : htlproof.
 
   Ltac tac :=
@@ -1137,7 +1140,10 @@ Section CORRECTNESS.
           match_states (RTL.State s f sp pc' (Registers.Regmap.set dst v rs) m) R2.
   Proof.
     intros s f sp pc rs m chunk addr args dst pc' a v H H0 H1 R1 MSTATE.
-    inv_state. inv_arr_access.
+    inv_state.
+
+    (* FIXME this tactic loops indefinitely *)
+    inv_arr_access.
 
     + (** Preamble *)
       invert MARR. inv CONST. crush.
@@ -1209,6 +1215,8 @@ Section CORRECTNESS.
 
       inversion NORMALISE_BOUND as [ NORMALISE_BOUND_LOW NORMALISE_BOUND_HIGH ];
       clear NORMALISE_BOUND.
+
+      (*
 
       (** Start of proof proper *)
       eexists. split.
@@ -1502,7 +1510,8 @@ Section CORRECTNESS.
       exact tt.
       exact (Values.Vint (Int.repr 0)).
       exact tt.
-  Qed.
+  *)
+  Admitted.
   Hint Resolve transl_iload_correct : htlproof.
 
   Lemma transl_istore_correct:
@@ -1568,7 +1577,7 @@ Section CORRECTNESS.
       eexists. split.
       eapply Smallstep.plus_one.
       eapply HTL.step_module; eauto.
-      econstructor. econstructor. econstructor.
+      econstructor. econstructor. econstructor. econstructor.
       eapply Verilog.stmnt_runp_Vnonblock_arr. crush.
       econstructor.
       econstructor.
@@ -1847,7 +1856,7 @@ Section CORRECTNESS.
       eexists. split.
       eapply Smallstep.plus_one.
       eapply HTL.step_module; eauto.
-      econstructor. econstructor. econstructor.
+      econstructor. econstructor. econstructor. econstructor.
       eapply Verilog.stmnt_runp_Vnonblock_arr. crush.
       econstructor.
       econstructor. econstructor. econstructor. econstructor.
@@ -2100,7 +2109,7 @@ Section CORRECTNESS.
       eexists. split.
       eapply Smallstep.plus_one.
       eapply HTL.step_module; eauto.
-      econstructor. econstructor. econstructor.
+      econstructor. econstructor. econstructor. econstructor.
       eapply Verilog.stmnt_runp_Vnonblock_arr. crush.
       econstructor. econstructor. econstructor. econstructor.
 
@@ -2338,7 +2347,7 @@ Section CORRECTNESS.
       eapply eval_cond_correct; eauto. intros.
       intros. eapply RTL.max_reg_function_use. apply H22. auto.
       econstructor. auto.
-      simpl. econstructor. unfold Verilog.merge_regs. unfold_merge. simpl.
+      simpl. econstructor. econstructor. unfold Verilog.merge_regs. unfold_merge. simpl.
       apply AssocMap.gss.
 
       inv MARR. inv CONST.
@@ -2355,7 +2364,7 @@ Section CORRECTNESS.
       eapply eval_cond_correct; eauto. intros.
       intros. eapply RTL.max_reg_function_use. apply H22. auto.
       econstructor. auto.
-      simpl. econstructor. unfold Verilog.merge_regs. unfold_merge. simpl.
+      simpl. econstructor. econstructor. unfold Verilog.merge_regs. unfold_merge. simpl.
       apply AssocMap.gss.
 
       inv MARR. inv CONST.
@@ -2408,7 +2417,7 @@ Section CORRECTNESS.
       econstructor; simpl; trivial.
       constructor.
       econstructor; simpl; trivial.
-      constructor.
+      constructor. constructor.
 
       constructor. constructor.
 
@@ -2434,7 +2443,7 @@ Section CORRECTNESS.
       eapply HTL.step_module; eauto.
       inv CONST; assumption.
       inv CONST; assumption.
-      constructor.
+      constructor. constructor.
       econstructor; simpl; trivial.
       econstructor; simpl; trivial.
       constructor. constructor. constructor.
